LeafImpl

Impl/LeafImpl.i.dfy
@@ -29,61 +29,60 @@ module LeafImpl {
     k2 := [] + k;
   }
 
-  method repivotLeaf(s: ImplVariables, ref: BT.G.Reference)
-  requires Inv(s)
-  requires s.ready
-  requires ref in s.ephemeralIndirectionTable.I().graph
-  requires s.cache.ptr(ref).Some?
-  requires s.cache.I()[ref].children.None?
-  requires |s.cache.I()[ref].buckets| == 1
-  requires |s.ephemeralIndirectionTable.I().graph| <= IT.MaxSize() - 1
-  modifies s.Repr()
+  method repivotLeaf(linear inout s: ImplVariables, ref: BT.G.Reference)
+  requires old_s.Inv()
+  requires old_s.ready
+  requires ref in old_s.ephemeralIndirectionTable.I().graph
+  requires old_s.cache.ptr(ref).Some?
+  requires old_s.cache.I()[ref].children.None?
+  requires |old_s.cache.I()[ref].buckets| == 1
+  requires |old_s.ephemeralIndirectionTable.I().graph| <= IT.MaxSize() - 1
   ensures s.ready
-  ensures WellUpdated(s)
-  ensures s.I() == LeafModel.repivotLeaf(old(s.I()), ref, old(s.cache.I()[ref]));
+  ensures s.W()
+  ensures s.I() == LeafModel.repivotLeaf(old_s.I(), ref, old_s.cache.I()[ref]);
   {
     LeafModel.reveal_repivotLeaf();
+    var b := false;
 
-    if s.frozenIndirectionTable != null {
-      var b := s.frozenIndirectionTable.HasEmptyLoc(ref);
-      if b {
-        print "giving up; repivotLeaf can't run because frozen isn't written";
-        return;
+    if s.frozenIndirectionTable.lSome? {
+      b := s.frozenIndirectionTable.value.HasEmptyLoc(ref);
+    }
+
+    if b {
+      print "giving up; repivotLeaf can't run because frozen isn't written";
+    } else {
+      var bounded := s.cache.NodeBoundedBucket(ref, ref, 0);
+      ghost var buckets := s.cache.I()[ref].buckets;
+      assert bounded == BoundedBucketList(buckets, s.cache.I()[ref].pivotTable);
+      if !bounded {
+        print "giving up; repivotLeaf can't run because current leaf is incorrect";
+      } else {
+        var pivot: KeyType.Key;
+        linear var left, right;
+        var pivots := InitPivotTable();
+
+        left, right, pivot := s.cache.NodeSplitMiddle(ref);
+        linear var buckets' := lseq_alloc(2);
+        lseq_give_inout(inout buckets', 0, left);
+        lseq_give_inout(inout buckets', 1, right);
+
+        pivot := CopyKey(pivot);
+        pivots := Insert(pivots, Keyspace.Element(pivot), 1);
+
+        linear var newnode := Node(pivots, None, buckets');
+        writeBookkeeping(inout s, ref, None);
+        inout s.cache.Insert(ref, newnode);
+        assert s.W();
+
+        ghost var a := s.I();
+        ghost var oldnode := old_s.cache.I()[ref];
+        ghost var b := LeafModel.repivotLeaf(old_s.I(), ref, oldnode);
+        assert newnode.I() == BT.G.Node(pivots, None, [
+              SplitBucketLeft(oldnode.buckets[0], pivot),
+              SplitBucketRight(oldnode.buckets[0], pivot)
+            ]);
+        assert a.cache == b.cache;
       }
     }
-
-    var bounded := s.cache.NodeBoundedBucket(ref, ref, 0);
-    ghost var buckets := s.cache.I()[ref].buckets;
-    assert bounded == BoundedBucketList(buckets, s.cache.I()[ref].pivotTable);
-    if !bounded {
-      print "giving up; repivotLeaf can't run because current leaf is incorrect";
-      return;
-    }
-
-    var pivot: KeyType.Key;
-    linear var left, right;
-    var pivots := InitPivotTable();
-
-    left, right, pivot := s.cache.NodeSplitMiddle(ref);
-    linear var buckets' := lseq_alloc(2);
-    lseq_give_inout(inout buckets', 0, left);
-    lseq_give_inout(inout buckets', 1, right);
-
-    pivot := CopyKey(pivot);
-    pivots := Insert(pivots, Keyspace.Element(pivot), 1);
-
-    linear var newnode := Node(pivots, None, buckets');
-    writeBookkeeping(s, ref, None);
-    s.cache.Insert(ref, newnode);
-    assert s.W();
-
-    ghost var a := s.I();
-    ghost var oldnode := old(s.cache.I()[ref]);
-    ghost var b := LeafModel.repivotLeaf(old(s.I()), ref, oldnode);
-    assert newnode.I() == old(BT.G.Node(pivots, None, [
-          SplitBucketLeft(oldnode.buckets[0], pivot),
-          SplitBucketRight(oldnode.buckets[0], pivot)
-        ]));
-    assert a.cache == b.cache;
   }
 }
